Phi_Semantics/PhiSem_Aggregate_Base.thy
@@ -445,6 +445,7 @@ ML_file \<open>syntax/index_param.ML\<close>
       Phi_Sys.set_param term (ctxt, @{thm Index_Param_Tag_Swap} RS sequent))\<close>
 *)
 
+
 section \<open>First-level Abstraction of Instructions\<close>
 
 lemma op_get_aggregate:
