Phi_System/Calculus_of_Programming.thy
@@ -419,7 +419,7 @@ lemma introduce_Ex_ToA_subj_P:
 paragraph \<open>Return\<close>
 
 
-lemma \<phi>M_Success[intro!]: (*depreciated?*)
+lemma \<phi>M_Success[intro!]: (*deprecated?*)
   \<open> v \<Turnstile> (y \<Ztypecolon> T)
 \<Longrightarrow> \<p>\<r>\<o>\<c> Return (\<phi>arg v) \<lbrace> X \<longmapsto> \<lambda>u. X\<heavy_comma> y \<Ztypecolon> Val u T \<rbrace> \<t>\<h>\<r>\<o>\<w>\<s> Any \<close>
   unfolding \<phi>Procedure_def det_lift_def Return_def
